almost done with liveness

liveness.v
@@ -4,11 +4,11 @@ Require Import FORYU.semantics.
 Require Import Orders.
 Require Import OrdersEx.
 Require Import MSets.
-Require Import MSetList.
 Require Import Arith.
+Require Import List.
+Import ListNotations.
 
-Open Scope nat_scope.
-
+Set Bullet Behavior "Strict Subproofs".
 
 Module VarSet := Make Nat_as_OT.
 
@@ -57,6 +57,155 @@ Module Liveness (D: DIALECT).
         end
     end.
 
+
+  Lemma remove_preserves_equal:
+    forall s1 s2 e,
+      VarSet.Equal s1 s2 ->
+      VarSet.Equal (VarSet.remove e s1) (VarSet.remove e s2).
+  Proof.
+    intros s1 s2 e Heq.
+    unfold VarSet.Equal in *.
+    intros x.
+    repeat rewrite VarSet.remove_spec.
+    rewrite Heq.
+    reflexivity.
+  Qed.
+
+  Lemma add_preserves_equal :
+    forall s1 s2 e,
+      VarSet.Equal s1 s2 ->
+      VarSet.Equal (VarSet.add e s1) (VarSet.add e s2).
+  Proof.
+    intros s1 s2 e Heq.
+    unfold VarSet.Equal in *.
+    intros x.
+    repeat rewrite VarSet.add_spec.
+    rewrite Heq.
+    reflexivity.
+  Qed.
+
+    Lemma mem_preserves_equal :
+    forall s1 s2 e,
+      VarSet.Equal s1 s2 ->
+      (VarSet.mem e s1) = (VarSet.mem e s2).
+  Proof.
+    intros s1 s2 e Heq.
+    unfold VarSet.Equal in *.
+    destruct (VarSet.mem e s1) eqn:H_mem_e_s1; destruct (VarSet.mem e s2) eqn:H_mem_e_s2; try reflexivity.
+   
+    + rewrite VarSet.mem_spec in H_mem_e_s1.
+      rewrite (Heq e) in H_mem_e_s1.
+      rewrite <- (VarSet.mem_spec s2 e) in H_mem_e_s1.
+      rewrite H_mem_e_s1 in H_mem_e_s2.
+      discriminate.
+
+    + rewrite VarSet.mem_spec in H_mem_e_s2.
+      rewrite <- (Heq e) in H_mem_e_s2.
+      rewrite <- (VarSet.mem_spec s1 e) in H_mem_e_s2.
+      rewrite H_mem_e_s2 in H_mem_e_s1.
+      discriminate.
+  Qed.
+      
+  Lemma apply_phi_preserves_equal:
+    forall l s1 s2,
+      VarSet.Equal s1 s2 ->
+      VarSet.Equal (apply_phi l s1) (apply_phi l s2).
+  Proof.
+    induction l as [|a l' IHl'].
+    + trivial.
+    + intros s1 s2 H_s1_eq_s2.
+      unfold apply_phi. fold apply_phi.
+      destruct a as [dest orig] eqn:E_do.
+      destruct orig as [var|] eqn:E_orig.
+      ++ pose proof (VarSet.mem_spec s1 dest) as H_mem_s1.
+         pose proof (VarSet.mem_spec s2 dest) as H_mem_s2.
+         destruct (VarSet.mem dest s1) eqn:E_mem_dest_s1;
+           destruct (VarSet.mem dest s2) eqn:E_mem_dest_s2.
+         +++ pose proof (add_preserves_equal (VarSet.remove dest s1) (VarSet.remove dest s2) var (remove_preserves_equal s1 s2 dest H_s1_eq_s2)) as H_add_rem_s1_s2_eq'.
+             apply IHl'.
+             apply H_add_rem_s1_s2_eq'.
+         +++ pose proof (remove_preserves_equal s1 s2 dest H_s1_eq_s2) as H_mem_s1_s2_dest.
+             rewrite <- VarSet.mem_spec in *.
+             pose proof (mem_preserves_equal s1 s2 dest H_s1_eq_s2) as H_mem_pre_eq.
+             rewrite H_mem_pre_eq in E_mem_dest_s1.
+             rewrite E_mem_dest_s1  in E_mem_dest_s2.
+             discriminate E_mem_dest_s2.
+         +++ pose proof (remove_preserves_equal s1 s2 dest H_s1_eq_s2) as H_mem_s1_s2_dest.
+             rewrite <- VarSet.mem_spec in *.
+             pose proof (mem_preserves_equal s1 s2 dest H_s1_eq_s2) as H_mem_pre_eq.
+             rewrite H_mem_pre_eq in E_mem_dest_s1.
+             rewrite E_mem_dest_s1  in E_mem_dest_s2.
+             discriminate E_mem_dest_s2.
+         +++ apply (IHl' s1 s2 H_s1_eq_s2).
+
+      ++ apply IHl'. apply H_s1_eq_s2.
+  Qed.
+
+  Lemma diff_preserves_equal:
+    forall s1 s1' s2 s2',
+      VarSet.Equal s1 s1' ->
+      VarSet.Equal s2 s2' ->
+      VarSet.Equal (VarSet.diff s1 s2) (VarSet.diff s1' s2').
+  Proof.
+    intros s1 s1' s2 s2' H_s1_eq_s1' H_s2_eq_s2'.
+    unfold VarSet.Equal in *.
+    intros x.
+    repeat rewrite VarSet.diff_spec.
+    rewrite H_s1_eq_s1'.
+    rewrite H_s2_eq_s2'.
+    reflexivity.
+  Qed.
+
+  Lemma union_preserves_equal:
+    forall s1 s1' s2 s2',
+      VarSet.Equal s1 s1' ->
+      VarSet.Equal s2 s2' ->
+      VarSet.Equal (VarSet.union s1 s2) (VarSet.union s1' s2').
+  Proof.
+    intros s1 s1' s2 s2' H_s1_eq_s1' H_s2_eq_s2'.
+    unfold VarSet.Equal in *.
+    intros x.
+    repeat rewrite VarSet.union_spec.
+    rewrite H_s1_eq_s1'.
+    rewrite H_s2_eq_s2'.
+    reflexivity.
+  Qed.
+
+  Lemma varset_equal_refl:
+    forall s,
+      VarSet.Equal s s.
+    Proof.
+      intro s.
+      unfold VarSet.Equal.
+      intros x.
+      reflexivity.
+    Qed.
+
+    Lemma varset_equal_sym:
+    forall s1 s2,
+      VarSet.Equal s1 s2 -> VarSet.Equal s2 s1.
+    Proof.
+      intros s1 s2 H_s1_eq_s2.
+      unfold VarSet.Equal in *.
+      intros x.
+      rewrite H_s1_eq_s2.
+      reflexivity.
+    Qed.
+
+    Lemma varset_equal_trans:
+    forall s0 s1 s2,
+      VarSet.Equal s0 s1 ->
+      VarSet.Equal s1 s2 ->
+      VarSet.Equal s0 s2.
+  Proof.
+    intros s0 s1 s H_s01 H_s12.
+    unfold VarSet.Equal in *.
+    intros x.
+    rewrite H_s01.
+    rewrite H_s12.
+    reflexivity.
+  Qed.
+
   Fixpoint prop_live_set_bkw (l: list InstructionD.t) (s: VarSet.t) : VarSet.t  :=
     match l with
     | nil => s
@@ -66,12 +215,43 @@ Module Liveness (D: DIALECT).
         let outset := list_to_set i.(InstructionD.output) in
         (VarSet.union (VarSet.diff s' outset) inset)
     end.
-  
+
+  Lemma prop_live_set_bkw_preserves_equal:
+        forall l s1 s2,
+          VarSet.Equal s1 s2 ->
+          VarSet.Equal (prop_live_set_bkw l s1) (prop_live_set_bkw l s2).
+  Proof.
+    induction l as [|a l' IHl'].
+    + trivial.
+    + intros s1 s2 H_s1_eq_s2.
+      unfold prop_live_set_bkw. fold prop_live_set_bkw.
+      apply (union_preserves_equal
+               (VarSet.diff (prop_live_set_bkw l' s1) (list_to_set (InstructionD.output a)))
+               (VarSet.diff (prop_live_set_bkw l' s2) (list_to_set (InstructionD.output a)))
+               (list_to_set (extract_yul_vars (InstructionD.input a)))
+               (list_to_set (extract_yul_vars (InstructionD.input a)))
+               (diff_preserves_equal (prop_live_set_bkw l' s1) (prop_live_set_bkw l' s2) (list_to_set (InstructionD.output a)) (list_to_set (InstructionD.output a)) (IHl' s1 s2 H_s1_eq_s2) (varset_equal_refl (list_to_set (InstructionD.output a))))
+               (varset_equal_refl (list_to_set (extract_yul_vars (InstructionD.input a))))).
+  Qed.
+
   Definition add_jump_var_if_applicable (b: BlockD.t) (s: VarSet.t) :=
     match b.(BlockD.exit_info) with
     | ExitInfoD.ConditionalJump cond_var _ _ => VarSet.add cond_var s
     | _ => s
       end.
+
+  Lemma add_jump_var_if_applicable_preserves_equal:
+    forall b s1 s2,
+      VarSet.Equal s1 s2 ->
+      VarSet.Equal (add_jump_var_if_applicable b s1) (add_jump_var_if_applicable b s2).
+  Proof.
+    intros b s1 s2 H_s1_eq_s2.
+    unfold add_jump_var_if_applicable.
+    destruct (BlockD.exit_info b); try apply H_s1_eq_s2.
+    rewrite (add_preserves_equal s1 s2 cond_var H_s1_eq_s2).
+    apply varset_equal_refl.
+    Qed.
+  
   
   (*
     Th  e following co-inductive defintions is for live variable properties.
@@ -82,46 +262,76 @@ Module Liveness (D: DIALECT).
   CoInductive live_out  (p : SmartContractD.t) : FunctionName.t -> BlockID.t -> VarSet.t -> Prop :=
 
   (* Return block *)
-  | lo_block_w_ret (fname : FunctionName.t) (bid :  BlockID.t) (b: BlockD.t) (rs: list SimpleExprD.t):
+  | lo_block_w_ret (fname : FunctionName.t) (bid :  BlockID.t) (b: BlockD.t) (rs: list SimpleExprD.t) (sout: VarSet.t):
     SmartContractD.get_block p fname bid = Some b -> (* the block exists *)
     BlockD.is_return_block b = Some rs -> (* it is an exit block and rs is the list of returned expressions *)
-    live_out p fname bid (list_to_set (extract_yul_vars rs))
+    VarSet.Equal sout (list_to_set (extract_yul_vars rs)) ->
+    live_out p fname bid sout
 
   (* Terminated block *)
-  | lo_block_w_ter (fname : FunctionName.t) (bid :  BlockID.t) (b: BlockD.t):
+  | lo_block_w_ter (fname : FunctionName.t) (bid :  BlockID.t) (b: BlockD.t) (sout: VarSet.t) :
     SmartContractD.get_block p fname bid = Some b -> (* the block exists *)
     BlockD.is_terminated_block b = true -> (* it is an terminate block *)
-    live_out p fname bid VarSet.empty 
+    VarSet.Equal sout VarSet.empty ->
+    live_out p fname bid sout
 
   (* A block with a with jump *)
-  | lo_block_w_jump (fname : FunctionName.t) (bid next_bid:  BlockID.t) (b next_b: BlockD.t) (s s': VarSet.t):
+  | lo_block_w_jump (fname : FunctionName.t) (bid next_bid:  BlockID.t) (b next_b: BlockD.t) (s: VarSet.t) (sout: VarSet.t):
     SmartContractD.get_block p fname bid = Some b -> (* the block exists *)
     BlockD.is_jump_block b = Some next_bid -> (* the block ends with a jump, and next_bid is the id of the next block *)
     live_in p fname next_bid s -> (* s is the set of live variables at the entry of p/fname/next_bid *)
     SmartContractD.get_block p fname next_bid = Some next_b -> (* next_b is the block with id next_bid *)
-    apply_phi (BlockD.phi_function next_b bid) s = s' -> (* apply -- in a reverse way -- the corresponding phi function on s to obain s' *)
-    live_out p fname bid s'  (* s' is the set of live variable at the exit of p/fname/bid *)
+    VarSet.Equal sout (apply_phi (BlockD.phi_function next_b bid) s) ->
+    live_out p fname bid sout  (* sout is the set of live variable at the exit of p/fname/bid *)
 
   (* A block with a conditional jump *)
-  | lo_block_w_cond_jump (fname : FunctionName.t) (bid next_bid_if_true next_bid_if_false:  BlockID.t) (cond_var: nat) (b next_b_if_true next_b_if_false: BlockD.t) (s1 s1' s2 s2': VarSet.t):
+  | lo_block_w_cond_jump (fname : FunctionName.t) (bid next_bid_if_true next_bid_if_false:  BlockID.t) (cond_var: nat) (b next_b_if_true next_b_if_false: BlockD.t) (s1 s2 sout: VarSet.t):
     SmartContractD.get_block p fname bid = Some b -> (* the block exists *)
     BlockD.is_cond_jump_block b = Some (cond_var, next_bid_if_true, next_bid_if_false) -> (* the block ends with a conditional jump, and next_bid_if_true and next_bid_if_false are the identifiers of the next blocks *)
     live_in p fname next_bid_if_true s1 ->  (* s1 is the set of live at the entry of p/fname/next_bid_if_true *)
     live_in p fname next_bid_if_false s2 -> (* s2 is the set of live variables at the entry of p/fname/next_bid_if_false *)
     SmartContractD.get_block p fname next_bid_if_true = Some next_b_if_true -> (* next_b_if_true is the block with id next_bid_if_true *)
     SmartContractD.get_block p fname next_bid_if_false = Some next_b_if_false -> (* next_b_if_false is the block with id next_bid_if_false *)
-    apply_phi (BlockD.phi_function next_b_if_true bid) s1 = s1' -> (* apply -- in a reverse way -- the corresponding phi function on s1 to obain s1' *)
-    apply_phi (BlockD.phi_function next_b_if_false bid) s2 = s2' -> (* apply -- in a reverse way -- the corresponding phi function on s2 to obain s2' *)
-    live_out p fname bid (VarSet.union s1' s2') (* s1' \/ s2' is the set of live at the exit ofx p/fname/bid *)
+    VarSet.Equal sout (VarSet.union (apply_phi (BlockD.phi_function next_b_if_true bid) s1) (apply_phi (BlockD.phi_function next_b_if_false bid) s2)) ->
+    live_out p fname bid sout
   with
     live_in (p : SmartContractD.t) : FunctionName.t -> BlockID.t -> VarSet.t -> Prop :=
-  | li_block_any (fname : FunctionName.t) (bid :  BlockID.t) (b: BlockD.t) (s: VarSet.t):
+  | li_block_any (fname : FunctionName.t) (bid :  BlockID.t) (b: BlockD.t) (s sout: VarSet.t):
     SmartContractD.get_block p fname bid = Some b -> (* the block exists *)
     live_out p fname bid s -> (* s is the set of live variables at the exit of p/fname/bid *)
-    live_in p fname bid (prop_live_set_bkw b.(BlockD.instructions) (add_jump_var_if_applicable b s)).
+    VarSet.Equal sout (prop_live_set_bkw b.(BlockD.instructions) (add_jump_var_if_applicable b s)) ->
+    live_in p fname bid sout.
 
+  Lemma live_in_varset_eq:
+    forall p f bid s1 s2,
+      VarSet.Equal s1 s2 ->
+      live_in p f bid s1 ->
+      live_in p f bid s2.
+  Proof.
+    intros p f bid s1 s2 H_s1_eq_s2 H_live_in_s1.
+    destruct H_live_in_s1.
+    apply (@li_block_any p fname bid b s s2 H H0 (varset_equal_trans s2 sout (prop_live_set_bkw (BlockD.instructions b) (add_jump_var_if_applicable b s)) (varset_equal_sym sout s2 H_s1_eq_s2) H1)).
+  Qed.
+    
+  Lemma live_out_varset_eq:
+    forall p f bid s1 s2,
+      VarSet.Equal s1 s2 ->
+      live_out p f bid s1 ->
+      live_out p f bid s2.
+  Proof.
+    intros p f bid s1 s2 H_s1_eq_s2 H_live_out_s1.
+    destruct H_live_out_s1 eqn:E_live_out.
+
+    + apply (@lo_block_w_ret p fname bid b rs s2 e e0 (varset_equal_trans s2 sout (list_to_set (extract_yul_vars rs)) (varset_equal_sym sout s2 H_s1_eq_s2) e1)).
+
+    + apply (@lo_block_w_ter p fname bid b s2 e e0 (varset_equal_trans s2 sout VarSet.empty (varset_equal_sym sout s2 H_s1_eq_s2) e1)).
+
+    + apply (@lo_block_w_jump p fname bid next_bid b next_b s s2 e e0 l e1 (varset_equal_trans s2 sout (apply_phi (BlockD.phi_function next_b bid) s) (varset_equal_sym sout s2 H_s1_eq_s2) e2)).
+
+    + apply (@lo_block_w_cond_jump p fname bid next_bid_if_true next_bid_if_false cond_var b next_b_if_true next_b_if_false s1 s0 s2 e e0 l l0 e1 e2 (varset_equal_trans s2 sout (VarSet.union (apply_phi (BlockD.phi_function next_b_if_true bid) s1) (apply_phi (BlockD.phi_function next_b_if_false bid) s0)) (varset_equal_sym sout s2 H_s1_eq_s2) e3)).
+  Qed.
+  
   (* The following types are used to define the result of a live-variable analysis *)
-
   Definition block_live_info_t := nat -> option VarSet.t.
   Definition fun_live_info_t := BlockID.t -> option (VarSet.t * VarSet.t).
   Definition sc_live_info_t := FunctionName.t -> option fun_live_info_t.
@@ -152,34 +362,34 @@ Module Liveness (D: DIALECT).
         f_info b.(BlockD.bid) = Some (b_in_info,b_out_info) /\ (* The live-variable information of the block exists *)
         match b.(BlockD.exit_info) with
         | ExitInfoD.Terminated =>
-            b_out_info = VarSet.empty 
+            VarSet.Equal b_out_info  VarSet.empty 
         | ExitInfoD.ReturnBlock rs => 
-            b_out_info = list_to_set (extract_yul_vars rs) 
+            VarSet.Equal b_out_info (list_to_set (extract_yul_vars rs))
         | ExitInfoD.Jump next_bid =>
             exists next_b next_b_in_info next_b_out_info,
             SmartContractD.get_block p f next_bid = Some next_b /\ 
               f_info next_bid = Some (next_b_in_info,next_b_out_info) /\
-              b_out_info = apply_phi (BlockD.phi_function next_b b.(BlockD.bid)) next_b_in_info
+              VarSet.Equal b_out_info (apply_phi (BlockD.phi_function next_b b.(BlockD.bid)) next_b_in_info)
         | ExitInfoD.ConditionalJump cond_var next_bid_if_true next_bid_if_false => 
             exists next_b_if_true next_b_ift_in_info next_b_ift_out_info next_b_if_false next_b_iff_in_info next_b_iff_out_info,
             SmartContractD.get_block p f next_bid_if_true = Some next_b_if_true /\ 
             SmartContractD.get_block p f next_bid_if_false = Some next_b_if_false /\ 
               f_info next_bid_if_true = Some (next_b_ift_in_info,next_b_ift_out_info) /\
               f_info next_bid_if_false = Some (next_b_iff_in_info,next_b_iff_out_info) /\
-              b_out_info = VarSet.union
-                             (apply_phi (BlockD.phi_function next_b_if_true b.(BlockD.bid)) next_b_ift_in_info)
-                             (apply_phi (BlockD.phi_function next_b_if_false b.(BlockD.bid)) next_b_iff_in_info)
+              VarSet.Equal b_out_info (VarSet.union
+                                         (apply_phi (BlockD.phi_function next_b_if_true b.(BlockD.bid)) next_b_ift_in_info)
+                                         (apply_phi (BlockD.phi_function next_b_if_false b.(BlockD.bid)) next_b_iff_in_info))
         end.
-
-  Definition snd_block_in_info (p : SmartContractD.t) (r: sc_live_info_t) (f: FunctionName.t) (b: BlockD.t) : Prop :=
+ 
+  Definition snd_block_in_info (r: sc_live_info_t) (f: FunctionName.t) (b: BlockD.t) : Prop :=
     exists f_info b_in_info b_out_info,
       (r f) = Some f_info /\ (* The live-variable information of the function exists *)
         f_info b.(BlockD.bid) = Some (b_in_info,b_out_info) /\ (* The live-variable information of the block exists *)
-        b_in_info = prop_live_set_bkw b.(BlockD.instructions) (add_jump_var_if_applicable b b_out_info).
+        VarSet.Equal b_in_info (prop_live_set_bkw b.(BlockD.instructions) (add_jump_var_if_applicable b b_out_info)).
   
   Definition snd_block_info (p : SmartContractD.t) (r: sc_live_info_t) (f: FunctionName.t) (b: BlockD.t)
     : Prop :=
-    snd_block_in_info p r f b /\ snd_block_out_info p r f b.
+    snd_block_in_info r f b /\ snd_block_out_info p r f b.
   
 
   Definition snd_all_blocks_info (p : SmartContractD.t) (r: sc_live_info_t) : Prop :=
@@ -194,9 +404,9 @@ Module Liveness (D: DIALECT).
   Proof.
     intros p f bid b H_exists.
     unfold SmartContractD.get_block in H_exists.
-    destruct (SmartContractD.get_function p f) as [|func]; try discriminate.
+    destruct (SmartContractD.get_function p f) as [func|]; try discriminate.
     unfold SmartContractD.FunctionD.get_block in H_exists.
-    destruct (find (fun b : SmartContractD.FunctionD.BlockD.t => BlockID.eqb (SmartContractD.FunctionD.BlockD.bid b) bid) (SmartContractD.FunctionD.blocks t)) as [|block] eqn:H_find; try discriminate.
+    destruct (find (fun b : SmartContractD.FunctionD.BlockD.t => BlockID.eqb (SmartContractD.FunctionD.BlockD.bid b) bid) (SmartContractD.FunctionD.blocks func)) as [block|] eqn:H_find; try discriminate.
     apply find_some in H_find.
     destruct H_find as [_ H_find].
     unfold BlockID.eqb in H_find.
@@ -275,20 +485,29 @@ Module Liveness (D: DIALECT).
       rewrite (bid_b p f bid b H_b_exists) in H_f_info'.
       
       assert (H_f_info_info': f_info = f_info').
-      {rewrite H_f_info in H_r_f. injection H_r_f as H_r_f. apply H_r_f. }.
+      (*{*)
+        rewrite H_f_info in H_r_f. injection H_r_f as H_r_f. apply H_r_f.
+      (*}*)
 
       assert (H_b_in_info_info': b_in_info = b_in_info').
-      {rewrite <- H_f_info_info' in H_f_info'. rewrite H_b_info in H_f_info'. injection H_f_info' as H_b_in_info_info' H_b_out_info_info'. rewrite H_b_in_info_info'. reflexivity.}.
+      (*{*)
+      rewrite <- H_f_info_info' in H_f_info'. rewrite H_b_info in H_f_info'. injection H_f_info' as H_b_in_info_info' H_b_out_info_info'. rewrite H_b_in_info_info'. reflexivity.
+      (*{*)
 
       assert (H_b_out_info_info': b_out_info = b_out_info').
-      {rewrite <- H_f_info_info' in H_f_info'. rewrite H_b_info in H_f_info'. injection H_f_info' as _ H_b_out_info_info'. rewrite H_b_out_info_info'. reflexivity.}.
+      (*{*)
+      rewrite <- H_f_info_info' in H_f_info'. rewrite H_b_info in H_f_info'. injection H_f_info' as _ H_b_out_info_info'. rewrite H_b_out_info_info'. reflexivity.
+      (*}*)
 
       rewrite H_b_in_info_info'.
-      rewrite H_b_in_info'.
-      apply (@li_block_any p f bid b b_out_info' H_b_exists).
+      rewrite <- H_b_out_info_info' in H_b_in_info'.
+
+      apply (@li_block_any p f bid b b_out_info' b_in_info' H_b_exists).
 
       apply (build_live_out p f bid b r f_info' b_in_info' b_out_info' H_snd_info H_b_exists H_r_f  H_f_info').
       
+      rewrite <- H_b_out_info_info'.
+      apply H_b_in_info'.            
         
     (* the case of live_out p f bid b_in_info *)
     - pose proof (H_snd_info f bid b H_b_exists) as H_snd_b_info.
@@ -299,13 +518,17 @@ Module Liveness (D: DIALECT).
       rewrite (bid_b p f bid b H_b_exists) in H_f_info'.
   
       assert (H_f_info_info': f_info = f_info').
-      {rewrite H_f_info in H_r_f. injection H_r_f as H_r_f. apply H_r_f.}.
+      (*{*)
+      rewrite H_f_info in H_r_f. injection H_r_f as H_r_f. apply H_r_f.
+      (*{*)
 
       rewrite (bid_b p f bid b H_b_exists) in H_b_out_info'.
 
       assert (H_b_out_info_info': b_out_info = b_out_info').
-      {rewrite <- H_f_info_info' in H_f_info'. rewrite H_b_info in H_f_info'. injection H_f_info' as _ H_b_out_info_info'. rewrite H_b_out_info_info'. reflexivity.}.
-            
+      (*{*)
+      rewrite <- H_f_info_info' in H_f_info'. rewrite H_b_info in H_f_info'. injection H_f_info' as _ H_b_out_info_info'. rewrite H_b_out_info_info'. reflexivity.
+      (*{*)
+             
       destruct b.(BlockD.exit_info) as [cond_var target_if_true target_if_false | target | return_values | ] eqn:E_exit_info.
 
       (* conditional jump *)
@@ -313,27 +536,22 @@ Module Liveness (D: DIALECT).
 
       rewrite H_b_out_info_info'.
       
-      rewrite H_b_out_info'.
-        
-      apply (@lo_block_w_cond_jump p f bid target_if_true target_if_false cond_var b next_b_if_true next_b_if_false next_b_ift_in_info (apply_phi (BlockD.phi_function next_b_if_true bid) next_b_ift_in_info) next_b_iff_in_info (apply_phi (BlockD.phi_function next_b_if_false bid) next_b_iff_in_info) H_b_exists (exit_info_vs_is_cond_jump b cond_var target_if_true target_if_false E_exit_info ) (build_live_in p f target_if_true next_b_if_true r f_info' next_b_ift_in_info next_b_ift_out_info H_snd_info H_b_next_ift_exists H_r_f H_f_ift_info') (build_live_in p f target_if_false next_b_if_false r f_info' next_b_iff_in_info next_b_iff_out_info H_snd_info H_b_next_iff_exists H_r_f H_f_iff_info') H_b_next_ift_exists H_b_next_iff_exists  eq_refl eq_refl).
+      apply  (@lo_block_w_cond_jump p f bid target_if_true target_if_false cond_var b next_b_if_true next_b_if_false next_b_ift_in_info next_b_iff_in_info b_out_info' H_b_exists (exit_info_vs_is_cond_jump b cond_var target_if_true target_if_false E_exit_info) (build_live_in p f target_if_true next_b_if_true r f_info' next_b_ift_in_info next_b_ift_out_info H_snd_info H_b_next_ift_exists H_r_f H_f_ift_info') (build_live_in p f target_if_false next_b_if_false r f_info' next_b_iff_in_info next_b_iff_out_info H_snd_info H_b_next_iff_exists H_r_f H_f_iff_info') H_b_next_ift_exists H_b_next_iff_exists H_b_out_info').
 
       (* jump *)
       + destruct H_b_out_info' as [next_b [next_b_in_info [next_b_out_info [H_b_next_exists [H_f_next_b_info' H_next_b_out_info']]]]].
 
       rewrite H_b_out_info_info'.
-      rewrite H_next_b_out_info'.
 
-      apply (@lo_block_w_jump p f bid target b next_b next_b_in_info (apply_phi (BlockD.phi_function next_b bid) next_b_in_info) H_b_exists (exit_info_vs_is_jump b target E_exit_info) (build_live_in p f target next_b r f_info' next_b_in_info next_b_out_info H_snd_info H_b_next_exists H_r_f H_f_next_b_info') H_b_next_exists eq_refl).      
+      apply (@lo_block_w_jump p f bid target b next_b next_b_in_info b_out_info' H_b_exists (exit_info_vs_is_jump b target E_exit_info) (build_live_in p f target next_b r f_info' next_b_in_info next_b_out_info H_snd_info H_b_next_exists H_r_f H_f_next_b_info') H_b_next_exists H_next_b_out_info').
 
       (* return *)
       + rewrite H_b_out_info_info'.
-        rewrite H_b_out_info'.
-        apply (@lo_block_w_ret p f bid b return_values H_b_exists (exit_info_vs_is_return b return_values E_exit_info)).
+        apply (@lo_block_w_ret p f bid b return_values b_out_info' H_b_exists (exit_info_vs_is_return b return_values E_exit_info ) H_b_out_info').
 
       (* teminated *)
       + rewrite H_b_out_info_info'.
-        rewrite H_b_out_info'.
-        apply (@lo_block_w_ter p f bid b H_b_exists (exit_info_vs_is_terminated b E_exit_info)).
+        apply (@lo_block_w_ter p f bid b b_out_info' H_b_exists (exit_info_vs_is_terminated b E_exit_info) H_b_out_info' ).
   Defined.
 
   Lemma snd_all_blocks_info_to_bid_info:
@@ -381,8 +599,418 @@ Module Liveness (D: DIALECT).
     - apply (build_live_out p f bid b r f_info b_in_info b_out_info H_snd_info H_b_exists H_r_f H_f_info).
   Qed.
     
+  Definition check_live_in (r: sc_live_info_t) (f: FunctionName.t) (b: BlockD.t) : bool :=
+    match (r f) with
+    | None => false
+    | Some f_info =>
+      match f_info b.(BlockD.bid) with
+      | None => false
+      | Some (b_in_info,b_out_info) =>
+          VarSet.equal b_in_info (prop_live_set_bkw b.(BlockD.instructions) (add_jump_var_if_applicable b b_out_info))
+      end
+    end.
+
+  Lemma check_live_in_snd:
+    forall r f b,
+      check_live_in r f b = true -> snd_block_in_info r f b.
+  Proof.
+    intros r f b H_check_live_in.
+    unfold check_live_in in H_check_live_in.
+    destruct (r f) as [f_info|] eqn:E_r_f; try discriminate.
+    destruct (f_info (BlockD.bid b)) as [b_info|] eqn:E_f_info_b; try discriminate.
+    destruct b_info as [b_in_info b_out_info].
+    unfold snd_block_in_info.
+    exists f_info. exists b_in_info. exists b_out_info.
+    split; try assumption.
+    split; try assumption.
+    rewrite <- VarSet.equal_spec.
+    apply H_check_live_in.
+  Qed.
+
+  Lemma check_live_in_complete:
+    forall r f b,
+      snd_block_in_info r f b -> check_live_in r f b = true.
+  Proof.
+    intros r f b H_snd.
+    unfold snd_block_in_info in H_snd.
+    destruct H_snd as [f_info [b_in_info [b_out_info [H_r_f [H_f_info H_eq]]]]].
+    unfold check_live_in.
+    destruct (r f) as [f_info'|]; try discriminate.
+    injection H_r_f as H_f_info_info'.
+    rewrite H_f_info_info'.
+    rewrite H_f_info.
+    rewrite VarSet.equal_spec.
+    apply H_eq.
+  Qed.
+
+  Lemma check_live_in_correct:
+    forall r f b,
+      snd_block_in_info r f b <-> check_live_in r f b = true.
+  Proof.
+    intros r f b.
+    split.
+    + apply check_live_in_complete.
+    + apply check_live_in_snd.
+  Qed.
+
+  Definition check_live_out (p: SmartContractD.t) (r: sc_live_info_t) (f: FunctionName.t) (b: BlockD.t) : bool :=
+    match (r f) with
+    | None => false
+    | Some f_info =>
+        match (f_info b.(BlockD.bid)) with
+        | None => false
+        | Some (b_in_info,b_out_info) =>
+            match b.(BlockD.exit_info) with
+            | ExitInfoD.Terminated =>
+                VarSet.equal b_out_info VarSet.empty 
+            | ExitInfoD.ReturnBlock rs => 
+                VarSet.equal b_out_info (list_to_set (extract_yul_vars rs))
+            | ExitInfoD.Jump next_bid =>
+                match (SmartContractD.get_block p f next_bid) with
+                | None => false
+                | Some next_b =>
+                    match (f_info next_bid) with
+                    | None => false
+                    | Some (next_b_in_info,next_b_out_info) =>
+                        VarSet.equal b_out_info (apply_phi (BlockD.phi_function next_b b.(BlockD.bid)) next_b_in_info)
+                    end
+                end
+            | ExitInfoD.ConditionalJump cond_var next_bid_if_true next_bid_if_false =>
+                match (SmartContractD.get_block p f next_bid_if_true) with
+                | None => false
+                | Some next_b_if_true =>
+                    match (SmartContractD.get_block p f next_bid_if_false) with
+                    | None => false
+                    | Some next_b_if_false =>
+                        match (f_info next_bid_if_true) with
+                        | None => false
+                        | Some (next_b_ift_in_info,next_b_ift_out_info) =>
+                            match (f_info next_bid_if_false) with
+                            | None => false
+                            | Some (next_b_iff_in_info,next_b_iff_out_info) =>
+                                VarSet.equal b_out_info (VarSet.union
+                                                           (apply_phi (BlockD.phi_function next_b_if_true b.(BlockD.bid)) next_b_ift_in_info)
+                                                           (apply_phi (BlockD.phi_function next_b_if_false b.(BlockD.bid)) next_b_iff_in_info))
+                            end
+                        end
+                    end
+                end
+            end
+        end
+    end.
+
+  Lemma check_live_out_snd:
+    forall p r f b,
+      check_live_out p r f b = true -> snd_block_out_info p r f b.
+  Proof.
+    intros p r f b H_check_live_out.
+    unfold check_live_out in H_check_live_out.
+    destruct (r f) as [f_info|] eqn:E_r_f; try discriminate.
+    destruct (f_info (BlockD.bid b)) as [b_info|] eqn:E_f_info_b; try discriminate.
+    destruct b_info as [b_in_info b_out_info].
+    unfold snd_block_out_info.
+    exists f_info. exists b_in_info. exists b_out_info.
+    split; try assumption.
+    split; try assumption.
+    destruct (BlockD.exit_info b) as [cond_var target_if_true target_if_false|next_bid|rs|] eqn:E_b_exit_info.
+
+    + destruct (SmartContractD.get_block p f target_if_true) as [next_b_if_true|]; try discriminate.
+      destruct (SmartContractD.get_block p f target_if_false) as [next_b_if_false|]; try discriminate.
+      destruct (f_info target_if_true) as [target_if_true_info|]; try discriminate.
+      destruct target_if_true_info as [next_b_ift_in_info next_b_ift_out_info].
+      destruct (f_info target_if_false) as [target_if_false_info|]; try discriminate.
+      destruct target_if_false_info as [next_b_iff_in_info next_b_iff_out_info].
+
+      exists next_b_if_true. exists next_b_ift_in_info. exists next_b_ift_out_info.
+      exists next_b_if_false. exists next_b_iff_in_info. exists next_b_iff_out_info.
+      split; try reflexivity.
+      split; try reflexivity.
+      split; try reflexivity.
+      split; try reflexivity.
+      rewrite <- VarSet.equal_spec.
+      apply H_check_live_out.
+
+    + destruct (SmartContractD.get_block p f next_bid) as [next_b|]; try discriminate.
+      destruct (f_info next_bid) as [next_bid_info|]; try discriminate.
+      destruct next_bid_info as [next_b_in_info next_b_out_info].
+      exists next_b. exists next_b_in_info. exists next_b_out_info.
+      split; try reflexivity.
+      split; try reflexivity.
+      rewrite <- VarSet.equal_spec.
+      apply H_check_live_out.
+
+    + rewrite <- VarSet.equal_spec.
+      apply H_check_live_out.
+
+    + rewrite <- VarSet.equal_spec.
+      apply H_check_live_out.
+  Qed.
+  
+Lemma check_live_out_complete:
+    forall p r f b,
+      snd_block_out_info p r f b -> check_live_out p r f b = true.
+  Proof.
+    intros p r f b H_snd.
+    unfold snd_block_out_info in H_snd.
+    destruct H_snd as [f_info [b_in_info [b_out_info [H_r_f [H_f_info H_eq]]]]].
+    unfold check_live_out.
+    rewrite H_r_f.
+    rewrite H_f_info.
+
+    destruct (BlockD.exit_info b) as [cond_var target_if_true target_if_false|next_bid|rs|] eqn:E_b_exit_info.
+
+    + destruct H_eq as [next_b_if_true [next_b_ift_in_info [next_b_ift_out_info [next_b_if_false [next_b_iff_in_info [next_b_iff_out_info [H_b_true_exists [H_b_false_exists [if_true_info [if_false_info H_eq]]]]]]]]]].
+
+      rewrite H_b_true_exists.
+      rewrite H_b_false_exists.
+      rewrite if_true_info.
+      rewrite if_false_info.
+      rewrite VarSet.equal_spec.
+      apply H_eq.
+
+    + destruct H_eq as [next_b [next_b_in_info [next_b_out_info [H_b_next_exists [H_next_b_f_info' H_eq]]]]].
+      rewrite H_b_next_exists.
+      rewrite H_next_b_f_info'.
+      rewrite VarSet.equal_spec.
+      apply H_eq.
+
+    + rewrite VarSet.equal_spec.
+      apply H_eq.
+    + rewrite VarSet.equal_spec.
+      apply H_eq.
+  Qed.
+  
+  Lemma check_live_out_correct:
+    forall p r f b,
+      snd_block_out_info p r f b <-> check_live_out p r f b = true.
+  Proof.
+    intros p r f b.
+    split.
+    + apply check_live_out_complete.
+    + apply check_live_out_snd.
+  Qed.
+
+  Definition check_live (p: SmartContractD.t) (r: sc_live_info_t) (f: FunctionName.t) (b: BlockD.t) : bool :=
+    if (check_live_in r f b) then check_live_out p r f b else false.
+
+  Lemma check_live_snd:
+    forall p r f b,
+      check_live p r f b = true -> snd_block_info p r f b.
+  Proof.
+    intros p r f b H_check_live.
+    unfold check_live in H_check_live.
+    destruct (check_live_in r f b) eqn:E_check_live; try discriminate.
+    unfold snd_block_info.
+    split.
+    + apply (check_live_in_snd r f b E_check_live).
+    + apply (check_live_out_snd p r f b H_check_live).
+  Qed.
+
+  Lemma check_live_complete:
+    forall p r f b,
+      snd_block_info p r f b -> check_live p r f b = true.
+  Proof.
+    intros p r f b H_snd.
+    unfold snd_block_info in H_snd.
+    destruct H_snd as [H_snd_in H_snd_out].
+    unfold check_live.
+    rewrite (check_live_in_complete r f b H_snd_in).
+    rewrite (check_live_out_complete p r f b H_snd_out).
+    reflexivity.
+  Qed.
+
+  Lemma check_live_correct:
+    forall p r f b,
+      snd_block_info p r f b <-> check_live p r f b = true.
+  Proof.
+    intros p r f b.
+    split.
+    + apply check_live_complete.
+    + apply check_live_snd.
+  Qed.
+      
+  Definition get_all_blocks (p: SmartContractD.t) :=
+    fold_right (fun f accm => (map (fun (b: BlockD.t) => (f.(FunctionD.name),b)) f.(FunctionD.blocks))++accm) nil p.(SmartContractD.functions).
+  
+  Lemma get_all_blocks_correct:
+    forall p l,
+      get_all_blocks p = l ->
+      forall fname b, In (fname,b) l <-> SmartContractD.get_block p fname b.(BlockD.bid) = Some b.
+  Admitted.
+  
+  Fixpoint forallb_stop {A : Type} (test : A -> bool) (l : list A) : bool :=
+    match l with
+    | [] => true
+    | x :: xs => if test x then forallb_stop test xs else false
+    end.
+  
+  Lemma forallb_stop_if:
+    forall (A: Type)  (P: A -> Prop ) (l: list A) (f: A->bool),
+      (forall x, ((f x) = true -> P x)) ->
+      (forallb_stop f l) = true ->
+      forall a, In a l -> P a.
+  Proof.
+    intros A P.
+    induction l as [| z l' IHl'].
+    + intros.
+      destruct H1.
+    + intros f H H_forallbs.
+      simpl in H_forallbs.
+      destruct (f z) eqn:E_f_z; try discriminate.
+      pose proof (H z E_f_z) as H_P_z.
+      intro a.
+      simpl.
+      intros H_disj.
+      destruct H_disj as [H_l | H_r].
+    - rewrite H_l in H_P_z.
+      apply H_P_z.
+    - apply (IHl' f H H_forallbs a H_r).
+  Qed.
+  
+  Lemma forallb_stop_fi:
+    forall (A: Type)  (P: A -> Prop ) (f: A->bool) (l: list A) ,
+      (forall a, In a l -> P a) ->
+      (forall a, (P a -> (f a) = true)) ->
+      (forallb_stop f l) = true.
+  Proof.
+    intros A P f.
+    induction l as [| z l' IHl'].
+    - reflexivity.
+    - intro H_P_a.
+      intro H_P_a_f_a.
+      simpl.
+      destruct (f z) eqn:E_f_z.      
+      + simpl in H_P_a.
+        assert (H_l': forall a : A, In a l' -> P a). intuition.
+        apply (IHl' H_l'  H_P_a_f_a).
+      + pose proof (H_P_a z (in_eq z l')) as H_P_z.
+        pose proof (H_P_a_f_a z H_P_z) as H_f_z_false.
+        rewrite H_f_z_false in E_f_z.
+        discriminate E_f_z.
+  Qed.
+  
+  Definition check_live_all_functions (p: SmartContractD.t) (r: sc_live_info_t) : bool :=
+    forallb_stop (fun i => check_live p r (fst i) (snd i)) (get_all_blocks p).
+  
+  Lemma aux:
+    forall p r i,
+      (check_live p r (fst i) (snd i) = true -> snd_block_info p r (fst i) (snd i)).
+  Proof.
+    intros p r i.
+    destruct i as [f b].
+    simpl.
+    apply (check_live_snd p r f b).
+  Qed.
+  
+  Lemma aux_aux:
+    forall p r i,
+      (snd_block_info p r (fst i) (snd i) -> check_live p r (fst i) (snd i) = true).
+  Proof.
+    intros p r i.
+    destruct i as [f b].
+    simpl.
+    apply (check_live_complete p r f b).
+  Qed.
+  
+  Lemma check_live_function_snd:
+    forall p r,
+      check_live_all_functions p r = true ->
+      snd_all_blocks_info p r.
+  Proof.
+    intros p r H_chk.
+    unfold check_live_all_functions in H_chk.
+    
+    pose proof (forallb_stop_if
+                  (FunctionName.t*BlockD.t)
+                  (fun i => snd_block_info p r (fst i) (snd i))
+                  (get_all_blocks p)
+                  (fun i => check_live p r (fst i) (snd i))
+                  (aux p r)
+                  H_chk).
+    
+    pose proof (get_all_blocks_correct p (get_all_blocks p) eq_refl).
+    
+    assert(H1: forall (fname : FunctionName.t) (b : BlockD.t),
+              SmartContractD.get_block p fname (BlockD.bid b) = Some b -> snd_block_info p r fname b).
+      (*{*)
+      intros fname b.
+      pose proof (H0 fname b).
+      pose proof (H (fname,b)).
+      rewrite H1 in H2.
+      simpl in H2.
+      apply H2.
+      (*}*)
+    
+    assert(H2: forall (fname : FunctionName.t) (b : BlockD.t) (bid: BlockID.t),
+              SmartContractD.get_block p fname bid = Some b -> snd_block_info p r fname b).
+      (*{*)
+      intros fname b bid H_exists.
+      pose proof (bid_b p fname bid b H_exists).
+      rewrite <- H2 in H_exists.
+      apply (H1 fname b H_exists).
+      (*}*)
+    
+    unfold snd_all_blocks_info.
+    intros f bid b.
+    apply (H2 f b bid).
+  Qed.
+
+
+  Lemma check_live_function_complete:
+    forall p r,
+      snd_all_blocks_info p r -> check_live_all_functions p r = true.
+  Proof.    
+    intros p r H_snd.
+    unfold snd_all_blocks_info in H_snd.
+    
+    pose proof (get_all_blocks_correct p (get_all_blocks p) eq_refl).
+ 
+    assert( forall a,
+              In a (get_all_blocks p) -> snd_block_info p r (fst a) (snd a)).
+    (*{*)
+      intros a.
+      pose proof (H (fst a) (snd a)).
+      rewrite <- surjective_pairing in H0.
+      rewrite H0.
+      pose proof (H_snd (fst a) (snd a).(BlockD.bid) (snd a)).
+      apply H1.
+    (*}*)
+
+      
+    assert ((forall a : FunctionName.t * BlockD.t,
+     (fun i : FunctionName.t * BlockD.t => snd_block_info p r (fst i) (snd i)) a ->
+     (fun i : FunctionName.t * BlockD.t => check_live p r (fst i) (snd i)) a = true)).
+    (*{*)
+      intro a.
+      pose proof (check_live_complete p r (fst a) (snd a)).
+      apply H1.
+    (*}*)
+
+    
+    pose proof (forallb_stop_fi
+                  (FunctionName.t*BlockD.t)
+                  (fun i => snd_block_info p r (fst i) (snd i))
+                  (fun i => check_live p r (fst i) (snd i))
+                  (get_all_blocks p)
+                  H0
+                  (aux_aux p r)).
+    
+    unfold check_live_all_functions.
+    apply H2.
+  Qed.
+
+  Lemma check_live_function_correct:
+    forall p r,
+      snd_all_blocks_info p r <-> check_live_all_functions p r = true.
+  Proof.
+    intros p r.
+    split.
+    - apply check_live_function_complete.
+    - apply check_live_function_snd.
+  Qed.
 
 End Liveness.
+
 
 
 
